operations/Linearize_multiple.thy
@@ -1,4 +1,4 @@
-theory Linearize
+theory Linearize_multiple
   imports "Binders.MRBNF_Composition" "Binders.MRBNF_Recursor"
 begin
 
@@ -12,27 +12,29 @@ to be pullback-preserving), we transform it into an MRBNF F' that has the same c
 as F except that the 3rd position becomes map-constrained to small-support endobijections.  
 *)
 
-typedecl ('a, 'b, 'c, 'd) F
+typedecl ('a, 'b, 'c, 'd, 'e) F
 consts map_F :: "('a :: var \<Rightarrow> 'a) \<Rightarrow> ('b :: var \<Rightarrow> 'b) \<Rightarrow>
-  ('c \<Rightarrow> 'c') \<Rightarrow> ('d \<Rightarrow> 'd') \<Rightarrow> ('a, 'b, 'c, 'd) F \<Rightarrow> ('a, 'b, 'c', 'd') F"
-consts set1_F :: "('a :: var, 'b :: var, 'c, 'd) F \<Rightarrow> 'a set"
-consts set2_F :: "('a :: var, 'b :: var, 'c, 'd) F \<Rightarrow> 'b set"
-consts set3_F :: "('a :: var, 'b :: var, 'c, 'd) F \<Rightarrow> 'c set"
-consts set4_F :: "('a :: var, 'b :: var, 'c, 'd) F \<Rightarrow> 'd set"
-consts rrel_F :: "('c \<Rightarrow> 'c' \<Rightarrow> bool) \<Rightarrow> ('d \<Rightarrow> 'd' \<Rightarrow> bool) \<Rightarrow> ('a :: var, 'b :: var, 'c, 'd) F \<Rightarrow> ('a, 'b, 'c', 'd') F \<Rightarrow> bool"
+  ('c \<Rightarrow> 'c') \<Rightarrow> ('d \<Rightarrow> 'd') \<Rightarrow> ('e \<Rightarrow> 'e') \<Rightarrow> ('a, 'b, 'c, 'd, 'e) F \<Rightarrow> ('a, 'b, 'c', 'd', 'e') F"
+consts set1_F :: "('a :: var, 'b :: var, 'c, 'd, 'e) F \<Rightarrow> 'a set"
+consts set2_F :: "('a :: var, 'b :: var, 'c, 'd, 'e) F \<Rightarrow> 'b set"
+consts set3_F :: "('a :: var, 'b :: var, 'c, 'd, 'e) F \<Rightarrow> 'c set"
+consts set4_F :: "('a :: var, 'b :: var, 'c, 'd, 'e) F \<Rightarrow> 'd set"
+consts set5_F :: "('a :: var, 'b :: var, 'c, 'd, 'e) F \<Rightarrow> 'e set"
+consts rrel_F :: "('c \<Rightarrow> 'c' \<Rightarrow> bool) \<Rightarrow> ('d \<Rightarrow> 'd' \<Rightarrow> bool) \<Rightarrow> ('e \<Rightarrow> 'e' \<Rightarrow> bool) \<Rightarrow> ('a :: var, 'b :: var, 'c, 'd, 'e) F 
+  \<Rightarrow> ('a, 'b, 'c', 'd', 'e') F \<Rightarrow> bool"
 
 declare [[mrbnf_internals]]
 declare [[typedef_overloaded]]
-mrbnf "('a :: var, 'b :: var, 'c, 'd) F"
+mrbnf "('a :: var, 'b :: var, 'c, 'd, 'e) F"
   map: map_F
-  sets: free: set1_F bound: set2_F live: set3_F live: set4_F
+  sets: free: set1_F bound: set2_F live: set3_F live: set4_F live: set5_F
   bd: natLeq
   rel: rrel_F
   var_class: var
   sorry
 
-(* we linearize this MRBNF on position 3*)
-ML \<open>val lin_pos = 3\<close>
+(* we linearize this MRBNF on position 3 and 5*)
+ML \<open>val lin_poses = [3, 5]\<close>
 
 print_mrbnfs
 declare [[ML_print_depth=10000]]
@@ -43,13 +45,13 @@ axiomatization where
    NB: All MRBNFs already preserve _weak_ pullbacks, i.e., they satisfy the following property 
    without uniqueness.  *)
   F_rel_map_set2_strong: 
-  "\<And> R S (x :: ('a :: var,'b :: var,'c,'d) F) y.
-    rrel_F R S x y =
-      (\<exists>!z. set3_F z \<subseteq> {(x, y). R x y} \<and>
-            set4_F z \<subseteq> {(x, y). S x y} \<and> map_F id id fst fst z = x \<and> map_F id id snd snd z = y)"
+  "\<And> R S T (x :: ('a :: var,'b :: var,'c,'d,'e) F) y.
+    rrel_F R S T x y =
+      (\<exists>!z. set3_F z \<subseteq> {(x, y). R x y} \<and> set4_F z \<subseteq> {(x, y). S x y} \<and>
+            set5_F z \<subseteq> {(x, y). T x y} \<and> map_F id id fst fst fst z = x \<and> map_F id id snd snd snd z = y)"
   and
   (* The next property assumes that nonrepetitive elements exist: *)
-  ex_nonrep: "\<exists>x. \<forall>x'. (\<exists> R. rrel_F R (=) x x') \<longrightarrow> (\<exists> f. x' = map_F id id f id x)"
+  ex_nonrep: "\<exists>x. \<forall>x'. (\<exists> R1 R2. rrel_F R1 (=) R2 x x') \<longrightarrow> (\<exists> f1 f2 . x' = map_F id id f1 id f2 x)"
 
 abbreviation "rel_F \<equiv> mr_rel_F"
 
@@ -112,53 +114,11 @@ fun mk_F_strong_tac mrbnf F_map_id mr_rel_F_def F_mr_rel_mono_strong0 F_rel_map_
   end
 \<close>
 
-(* lin_pos independent *)
 lemma F_strong:
-  "rel_F id id R3 R4 x y \<Longrightarrow> rel_F id id Q3 Q4 x y \<Longrightarrow> rel_F id id (inf R3 Q3) (inf R4 Q4) x y"
-  apply (tactic \<open>mk_F_strong_tac (MRBNF_Def.mrbnf_of @{context} @{type_name F} |> the) @{thm F.map_id} 
+  "rel_F id id R3 R4 R5 x y \<Longrightarrow> rel_F id id Q3 Q4 Q5 x y \<Longrightarrow> rel_F id id (inf R3 Q3) (inf R4 Q4) (inf R5 Q5) x y"
+  by (tactic \<open>mk_F_strong_tac (MRBNF_Def.mrbnf_of @{context} @{type_name F} |> the) @{thm F.map_id} 
     @{thm mr_rel_F_def} @{thm F.mr_rel_mono_strong0} @{thm F_rel_map_set2_strong} @{thm F.in_rel} @{context} 
-    THEN print_tac @{context} "done" THEN no_tac\<close>)
-
-  apply (frule F.mr_rel_mono_strong0[OF supp_id_bound bij_id supp_id_bound supp_id_bound bij_id supp_id_bound];
-      ((rule ballI, rule ballI refl)?, 
-        (rule impI, rule trans[OF top_apply[THEN fun_cong] trans[OF top_apply top_bool_def]])?))
-  apply(rotate_tac 2)
-  apply (unfold F.map_id mr_rel_F_def eq_True)
-  thm F_rel_map_set2_strong
-  apply (drule F_rel_map_set2_strong[THEN iffD1])
-  apply (unfold top_apply top_bool_def Collect_const_case_prod if_True eqTrueI[OF subset_UNIV] simp_thms(22))
-  apply (unfold F.in_rel[OF supp_id_bound bij_id supp_id_bound, unfolded id_apply F.map_id OO_Grp_alt]
-      id_def[symmetric] mem_Collect_eq)
-  apply (elim exE alt_ex1E)
-  apply (erule conjE)
-  apply (erule conjE)
-  apply (erule conjE)
-  apply (erule conjE)
-  apply (erule conjE)
-  apply (erule conjE)
-  apply (erule conjE)
-  subgoal premises subprems for z l r
-    thm subprems
-    apply (insert spec2[OF subprems(1), of r z]
-        spec2[OF subprems(1), of l z]; (erule impE); (erule impE))
-       apply (rule conjI; rule conjI; rule subprems)
-       apply (rule conjI; rule conjI; rule subprems)
-       apply (rule conjI; rule conjI; rule subprems)
-    apply (rule exI)
-    apply (unfold inf_fun_def inf_bool_def)
-    apply (rule conjI)
-     apply (insert subprems) []
-     apply (hypsubst_thin)
-    apply ((rule conjI)?,
-        rule subrelI, 
-        rule CollectI, 
-        rule case_prodI, 
-        (rule conjI; erule rev_subsetD[THEN iffD1[OF prod_in_Collect_iff]]),
-        assumption, assumption)+
-    apply (rule conjI)
-    apply (rule subprems)+
-    done
-  done
+    THEN print_tac @{context} "done"\<close>)
 
 ML \<open>
 open BNF_Util BNF_Tactics
@@ -189,145 +149,43 @@ fun mk_rel_F_exchange_tac mrbnf F_mr_rel_mono_strong0 F_strong ctxt =
 (* Another important consequence: the following "exchange"-property, which could be read: 
 Since the atoms have a fixed position, we can permute the relations: *)
 lemma rel_F_exchange: 
-  fixes x :: "('a1::var,'a2::var,'a3,'a4) F" and x' :: "('a1,'a2,'a3','a4') F"
-  assumes "rel_F id id R3 R4 x x'" and "rel_F id id Q3 Q4 x x'"
-  shows "rel_F id id R3 Q4 x x'" 
+  fixes x :: "('a1::var,'a2::var,'a3,'a4,'a5) F" and x' :: "('a1,'a2,'a3','a4','a5') F"
+  assumes "rel_F id id R3 R4 R5 x x'" and "rel_F id id Q3 Q4 Q5 x x'"
+  shows "rel_F id id R3 Q4 R5 x x'" 
   using assms apply -
-  apply (tactic \<open>mk_rel_F_exchange_tac (MRBNF_Def.mrbnf_of @{context} @{type_name F} |> the) 
+  by (tactic \<open>mk_rel_F_exchange_tac (MRBNF_Def.mrbnf_of @{context} @{type_name F} |> the) 
     @{thm F.mr_rel_mono_strong0} @{thm F_strong} @{context} 
-    THEN print_tac @{context} "done" THEN no_tac\<close>)
-  subgoal premises prems
-    apply (rule F.mr_rel_mono_strong0[OF supp_id_bound bij_id supp_id_bound supp_id_bound bij_id supp_id_bound])
-    apply (rule F_strong[OF prems])
-       apply (unfold id_apply eqTrueI[OF refl] ball_triv inf_apply inf_bool_def)
-       apply (intro impI TrueI)+
-     apply (intro ballI impI; erule conjunct1 conjunct2)+
-    done
-  done
+    THEN print_tac @{context} "done"\<close>)
 
 (* Then notion of two items having the same shape (w.r.t. the 3rd position): *)
 (* these definitions are lin_pos dependent *)
-definition sameShape1 :: "('a1::var,'a2::var,'a3,'a4) F \<Rightarrow> ('a1,'a2,'a3,'a4) F \<Rightarrow> bool" where 
-  "sameShape1 x x' \<equiv> \<exists> R. rel_F id id R (=) x x'"
+definition sameShape1 :: "('a1::var,'a2::var,'a3,'a4,'a5) F \<Rightarrow> ('a1,'a2,'a3,'a4,'a5) F \<Rightarrow> bool" where 
+  "sameShape1 x x' \<equiv> \<exists> R1 R2. rel_F id id R1 (=) R2 x x'"
 
-definition nonrep2 :: "('a1::var,'a2::var,'a3,'a4) F \<Rightarrow> bool" where 
-  "nonrep2 x \<equiv> \<forall> x'. sameShape1 x x' \<longrightarrow> (\<exists> f. x' = map_F id id f id x)"
-
-ML\<open>
-open BNF_Util BNF_Tactics
-
-fun mk_nonrep2_map_F_tac mrbnf nonrep_def sameShape_def F_map_comp F_mr_rel_map mr_rel_F_def F_rel_compp 
-  F_rel_Grp F_map_id F_in_rel F_rel_maps F_rel_refl_strong ctxt = 
-  HEADGOAL (Subgoal.FOCUS 
-    (fn {prems, context = ctxt, ...} => 
-      let
-        val var_types = var_types_of_mrbnf mrbnf;
-        val nr_lives = length (filter (fn v => v = MRBNF_Def.Live_Var) var_types);
-        val nr_non_lives = length (filter (fn v => not (v = MRBNF_Def.Live_Var)) var_types);
-        val lin_live_pos = fold_index (fn (i, v) => fn b => 
-          if (v = MRBNF_Def.Live_Var andalso i+1 < lin_pos) then b+1 else b) var_types 1;
-        val switch_poses = map_range (fn i => if i < (lin_pos-(lin_live_pos)) then i+1 else i+2) (nr_non_lives);
-        val switch = (fn thm1 => (fn thm2 => trans OF [thm1, thm2 RS sym]));
-        val o_id = @{thm o_id};
-        val id_o = @{thm id_o};
-      in
-        unfold_thms_tac ctxt [nonrep_def, sameShape_def] THEN
-        HEADGOAL (EVERY' [
-          rtac ctxt allI,
-          rtac ctxt impI,
-          etac ctxt exE,
-          EqSubst.eqsubst_tac ctxt [0] [F_map_comp] THEN_ALL_NEW
-            TRY o resolve_tac ctxt (prems @ @{thms supp_id_bound bij_id}),
-          K (unfold_thms_tac ctxt [switch id_o o_id]),
-          EqSubst.eqsubst_tac ctxt [lin_pos] [switch o_id id_o], (*move all id to the right except for lin_pos*)
-          EqSubst.eqsubst_tac ctxt [0] [F_map_comp RS sym] THEN_ALL_NEW
-            TRY o resolve_tac ctxt (prems @ @{thms supp_id_bound bij_id}),
-          dtac ctxt (rotate_prems ~1 (F_mr_rel_map RS iffD1)) THEN_ALL_NEW
-            TRY o resolve_tac ctxt (prems @ @{thms supp_id_bound bij_id}),
-          K (unfold_thms_tac ctxt [switch id_o o_id, @{thm Grp_UNIV_id}]),
-          K (unfold_thms_tac ctxt [switch @{thm OO_eq} @{thm eq_OO}]),  
-          EqSubst.eqsubst_asm_tac ctxt [lin_live_pos] [switch @{thm eq_OO} @{thm OO_eq}], (*move all (=) to the left except for lin_live_pos*)
-          K (unfold_thms_tac ctxt @{thms eq_alt}),   
-          EqSubst.eqsubst_tac ctxt [0] @{thms Grp_UNIV_id}
-        ]) THEN
-        unfold_thms_tac ctxt [mr_rel_F_def, o_id, F_rel_compp, F_rel_Grp] THEN
-        unfold_thms_tac ctxt [eqTrueI OF @{thms subset_UNIV}, @{thm simp_thms(21)}, id_o, @{thm UNIV_def} RS sym] THEN
-        unfold_thms_tac ctxt ([eqTrueI OF [@{thm UNIV_I}], id_apply] @ @{thms Grp_UNIV_id OO_def Grp_def simp_thms(21)}) THEN
-        HEADGOAL (EVERY' [
-          etac ctxt exE,
-          etac ctxt conjE,
-          dtac ctxt (rotate_prems ~1 (F_in_rel RS iffD1)) THEN_ALL_NEW
-            TRY o resolve_tac ctxt prems,
-          Method.insert_tac ctxt [unfold_thms ctxt [nonrep_def, sameShape_def, mr_rel_F_def, F_map_id] 
-            (nth prems (length prems -1))],
-          etac ctxt exE,
-          etac ctxt conjE,
-          etac ctxt CollectE,
-          etac ctxt conjE
-        ]) THEN
-        REPEAT_DETERM_N (nr_lives-1) (HEADGOAL (
-          etac ctxt conjE)) THEN
-        HEADGOAL (hyp_subst_tac_thin true ctxt) THEN
-        HEADGOAL (Subgoal.FOCUS 
-          (fn {prems = subprems, context = ctxt, params, ...} => 
-            HEADGOAL (EVERY' [
-              Method.insert_tac ctxt [nth subprems 0],
-              etac ctxt allE,
-              etac ctxt impE,
-              rtac ctxt (infer_instantiate' ctxt [NONE, SOME (snd (nth params 1))] exI),
-              EqSubst.eqsubst_tac ctxt [1] [nth F_rel_maps 0],
-              EqSubst.eqsubst_tac ctxt [1] [nth F_rel_maps 1]
-            ]) THEN
-            HEADGOAL (rtac ctxt F_rel_refl_strong) THEN
-            REPEAT_DETERM_N nr_lives (HEADGOAL (
-                (dresolve_tac ctxt (map (fn p => subsetD OF [p] RS @{thm Collect_case_prodD}) (drop 1 subprems)) THEN'
-                  (assume_tac ctxt ORELSE' 
-                  (rtac ctxt sym THEN' assume_tac ctxt))))) THEN
-            HEADGOAL (EVERY' [
-              etac ctxt exE,
-              EqSubst.eqsubst_tac ctxt [0] [F_map_comp] THEN_ALL_NEW
-                TRY o resolve_tac ctxt (prems @ @{thms supp_id_bound bij_id}),
-              EqSubst.eqsubst_tac ctxt switch_poses [switch id_o o_id],
-              EqSubst.eqsubst_tac ctxt [0] [F_map_comp RS sym] THEN_ALL_NEW
-                TRY o resolve_tac ctxt (prems @ @{thms supp_id_bound bij_id}),
-              rtac ctxt exI,
-              dtac ctxt arg_cong,
-              assume_tac ctxt
-            ]) 
-          ) ctxt)
-      end)
-  ctxt)
-\<close>
+definition nonrep2 :: "('a1::var,'a2::var,'a3,'a4,'a5) F \<Rightarrow> bool" where 
+  "nonrep2 x \<equiv> \<forall> x'. sameShape1 x x' \<longrightarrow> (\<exists> f1 f2. x' = map_F id id f1 id f2 x)"
 
 (* lin_pos dependent *)
 lemma nonrep2_map_F:
-  fixes x :: "('a1::var,'a2::var,'a3,'a4) F"
+  fixes x :: "('a1::var,'a2::var,'a3,'a4,'a5) F"
     and v :: "'a1 \<Rightarrow> 'a1" and u :: "'a2\<Rightarrow>'a2" and g :: "'a4 \<Rightarrow> 'b4"
   assumes v: "|supp v| <o |UNIV :: 'a1 set|"  and u: "bij u" "|supp u| <o |UNIV :: 'a2 set|" 
   assumes "nonrep2 x"
-  shows "nonrep2 (map_F v u id g x)"
+  shows "nonrep2 (map_F v u id g id x)"
   using assms apply -
-  apply (tactic \<open>mk_nonrep2_map_F_tac (MRBNF_Def.mrbnf_of @{context} @{type_name F} |> the) @{thm nonrep2_def} @{thm sameShape1_def} @{thm F.map_comp} 
-    @{thm F.mr_rel_map(1)} @{thm mr_rel_F_def} @{thm F.rel_compp} @{thm F.rel_Grp} @{thm F.map_id}
-    @{thm F.in_rel} @{thms F.rel_map} @{thm F.rel_refl_strong}
-    @{context}
-    THEN print_tac @{context} "done" THEN no_tac\<close>)
   subgoal premises prems
     apply (unfold nonrep2_def sameShape1_def)
     apply (rule allI)
     apply (rule impI)
     apply (elim exE)
     apply (subst F.map_comp; (rule prems bij_id supp_id_bound)?)
-    apply (unfold o_id id_o)
-    apply (subst F.map_comp[of id id _ _ id _ _ id, unfolded o_id id_o, symmetric]; (rule prems bij_id supp_id_bound)?)
-(*
     apply (unfold trans[OF id_o o_id[symmetric]])
-    apply (subst (3) trans[OF o_id id_o[symmetric]])
-    apply (subst F.map_comp[THEN sym]; (rule prems bij_id supp_id_bound)?)*)
+    apply (subst (3 5) trans[OF o_id id_o[symmetric]])
+    apply (subst F.map_comp[THEN sym]; (rule prems bij_id supp_id_bound)?)
     apply (drule iffD1[OF F.mr_rel_map(1), rotated -1]; (rule prems bij_id supp_id_bound)?)
     apply (unfold trans[OF id_o o_id[symmetric]] Grp_UNIV_id)
     apply (unfold trans[OF OO_eq eq_OO[symmetric]])
-    apply (subst (asm) (1) trans[OF eq_OO OO_eq [symmetric]])
+    apply (subst (asm) (1 3) trans[OF eq_OO OO_eq [symmetric]])
     apply (unfold eq_alt)
     apply (subst Grp_UNIV_id)
     apply (unfold mr_rel_F_def o_id F.rel_compp F.rel_Grp)
@@ -342,149 +200,64 @@ lemma nonrep2_map_F:
     apply (erule CollectE)
     apply (erule conjE)
     apply (erule conjE)
+    apply (erule conjE)
     apply (hypsubst_thin)
-    subgoal premises subprems for x' R y z
+    subgoal premises subprems for x' R1 R2 y z
+      thm subprems
       apply (insert subprems(1))
       apply (erule allE)
       apply (erule impE)
 (* this instantiation of R is not really necessary, but it feels better to have it concretely *)
-       apply (rule exI[of _ R])
+       apply (rule exI[of _ R1])
+       apply (rule exI[of _ R2]) (*repeat for each lin_pos*)
       apply (subst F.rel_map)
        apply (subst F.rel_map)
        apply (rule F.rel_refl_strong)
-         apply (drule subsetD[OF subprems(2), THEN Collect_case_prodD] subsetD[OF subprems(3), THEN Collect_case_prodD]; 
+         apply (drule subsetD[OF subprems(2), THEN Collect_case_prodD] 
+            subsetD[OF subprems(3), THEN Collect_case_prodD]
+            subsetD[OF subprems(4), THEN Collect_case_prodD]; 
                 (assumption)?; (rule sym; assumption)?)+
       apply (elim exE)
       apply (subst F.map_comp; (rule prems bij_id supp_id_bound)?)
       apply (subst (1 2) trans[OF id_o o_id[symmetric]])
       apply (subst F.map_comp[THEN sym]; (rule prems bij_id supp_id_bound)?)
       apply (rule exI)
+      apply (rule exI) (*repeat for each lin_pos*)
       apply (drule arg_cong)
       apply (assumption)
       done
     done
   done
 
-ML\<open>
-open BNF_Util BNF_Tactics
-
-fun mk_nonrep2_map_F_rev_tac mrbnf nonrep_def sameShape_def F_mr_rel_map1 F_mr_rel_map2 F_mr_rel_map3 F_map_comp F_rel_eq 
-  F_mr_rel_id rel_F_exchange F_mr_rel_flip F_mr_rel_mono_strong0 F_mr_rel_Grp ctxt = 
-  HEADGOAL (Subgoal.FOCUS 
-    (fn {prems, context = ctxt, ...} => 
-      let
-        val var_types = var_types_of_mrbnf mrbnf;
-        val nr_lives = length (filter (fn v => v = MRBNF_Def.Live_Var) var_types);
-        val nr_non_lives = length (filter (fn v => not (v = MRBNF_Def.Live_Var)) var_types);
-        val lin_live_pos = fold_index (fn (i, v) => fn b => 
-          if (v = MRBNF_Def.Live_Var andalso i+1 < lin_pos) then b+1 else b) var_types 1;
-        val switch = (fn thm1 => (fn thm2 => trans OF [thm1, thm2 RS sym]));
-      in
-        unfold_thms_tac ctxt [nonrep_def, sameShape_def] THEN
-        HEADGOAL (EVERY' [
-          rtac ctxt allI,
-          rtac ctxt impI,
-          etac ctxt exE,
-          forward_tac ctxt [rotate_prems ~1 F_mr_rel_map2] THEN_ALL_NEW
-            TRY o resolve_tac ctxt (prems @ @{thms supp_id_bound bij_id}),
-          rotate_tac 1,
-          EqSubst.eqsubst_asm_tac ctxt (map_range (fn i => i+1) nr_non_lives) [switch @{thm o_id} @{thm id_o}],
-          EqSubst.eqsubst_asm_tac ctxt [lin_live_pos] @{thms Grp_UNIV_id},
-          K (unfold_thms_tac ctxt [switch @{thm eq_OO} @{thm OO_eq}]),
-          EqSubst.eqsubst_asm_tac ctxt [lin_live_pos] [switch @{thm OO_eq} @{thm eq_OO}], (*move all (=) to the right and then lin_live_pos back*)
-          EqSubst.eqsubst_asm_tac ctxt [lin_live_pos] @{thms eq_alt},
-          EqSubst.eqsubst_asm_tac ctxt [0] [F_mr_rel_map1 RS sym] THEN_ALL_NEW
-            TRY o resolve_tac ctxt (prems @ @{thms supp_id_bound bij_id}),
-          Method.insert_tac ctxt [unfold_thms ctxt [nonrep_def, sameShape_def] (nth prems (length prems - 1))],
-          etac ctxt allE,
-          etac ctxt impE,
-          rtac ctxt exI,
-          assume_tac ctxt,
-          etac ctxt thin_rl,
-          etac ctxt exE,
-          EqSubst.eqsubst_asm_tac ctxt [0] [F_map_comp] THEN_ALL_NEW
-            TRY o resolve_tac ctxt (prems @ @{thms supp_id_bound bij_id}),
-          K (unfold_thms_tac ctxt @{thms id_o o_id}),
-          EqSubst.eqsubst_asm_tac ctxt [1] [F_rel_eq RS sym],
-          EqSubst.eqsubst_asm_tac ctxt [1] [F_mr_rel_id],
-          dtac ctxt (rotate_prems ~1 (iffD1 OF [F_mr_rel_map1])) THEN_ALL_NEW
-            TRY o resolve_tac ctxt (prems @ @{thms supp_id_bound bij_id}),
-          K (unfold_thms_tac ctxt @{thms id_o OO_eq}),
-          dtac ctxt (rotate_prems 1 rel_F_exchange),
-          rtac ctxt (F_mr_rel_flip RS iffD1) THEN_ALL_NEW
-            TRY o resolve_tac ctxt @{thms supp_id_bound bij_id},
-          K (unfold_thms_tac ctxt @{thms inv_id}),
-          EqSubst.eqsubst_asm_tac ctxt [0] [F_mr_rel_map3] THEN_ALL_NEW
-            TRY o resolve_tac ctxt (prems @ @{thms supp_id_bound bij_id}),
-          EqSubst.eqsubst_asm_tac ctxt (map_range (fn i => i+1) (2 * nr_lives)) @{thms Grp_def},
-          EqSubst.eqsubst_asm_tac ctxt (map_range (fn i => i+1) (nr_non_lives)) @{thms inv_o_simp1} THEN_ALL_NEW
-            TRY o resolve_tac ctxt (@{thm bij_id}::prems),
-          K (unfold_thms_tac ctxt ((eqTrueI OF @{thms UNIV_I}):: @{thms id_apply simp_thms(21)})),
-          EqSubst.eqsubst_asm_tac ctxt [lin_live_pos] @{thms eq_commute},
-          K (unfold_thms_tac ctxt @{thms eq_OO conversep_def}),
-          etac ctxt (rotate_prems (~1 - (length var_types)) F_mr_rel_mono_strong0) THEN_ALL_NEW
-            TRY o resolve_tac ctxt @{thms supp_id_bound bij_id}
-        ]) THEN
-        REPEAT_DETERM_N (length var_types) (
-          (HEADGOAL (
-            (* for bound and free *)
-            rtac ctxt ballI THEN'
-            rtac ctxt refl)) 
-          ORELSE 
-          (HEADGOAL (
-            (* for lives*)
-            rtac ctxt ballI THEN'
-            rtac ctxt ballI THEN'
-            rtac ctxt impI THEN'
-            rotate_tac 2 THEN'
-            EqSubst.eqsubst_asm_tac ctxt [0] @{thms eq_commute} THEN'
-            assume_tac ctxt))
-        ) THEN
-        HEADGOAL (EVERY' [
-          etac ctxt thin_rl,
-          EqSubst.eqsubst_asm_tac ctxt [lin_live_pos] [@{thm Grp_UNIV_def} RS sym],
-          rtac ctxt exI,
-          EqSubst.eqsubst_asm_tac ctxt (map_range (fn i => i+1) (nr_lives -1)) @{thms eq_alt},
-          EqSubst.eqsubst_asm_tac ctxt [0] [F_mr_rel_Grp] THEN_ALL_NEW
-            TRY o resolve_tac ctxt @{thms supp_id_bound bij_id}
-        ]) THEN
-        unfold_thms_tac ctxt ([eqTrueI OF @{thms subset_UNIV}, eqTrueI OF @{thms UNIV_I}, @{thm UNIV_def} RS sym] @ 
-          @{thms simp_thms(21) Grp_def}) THEN
-        HEADGOAL (assume_tac ctxt)
-      end)
-  ctxt)
-\<close>
-
 (* Here we need pullback preservation: *)
 lemma nonrep2_map_F_rev:
-  fixes x :: "('a1::var,'a2::var,'a3,'a4) F" and u :: "'a2\<Rightarrow>'a2" and g :: "'a4 \<Rightarrow> 'a4'"
+  fixes x :: "('a1::var,'a2::var,'a3,'a4,'a5) F" and u :: "'a2\<Rightarrow>'a2" and g :: "'a4 \<Rightarrow> 'a4'"
   assumes u: "bij u" "|supp u| <o |UNIV :: 'a2 set|" 
-  assumes "nonrep2 (map_F id u id g x)"
+  assumes "nonrep2 (map_F id u id g id x)"
   shows "nonrep2 x"
   using assms apply -
- (* apply (tactic \<open>mk_nonrep2_map_F_rev_tac (MRBNF_Def.mrbnf_of @{context} @{type_name F} |> the) @{thm nonrep2_def} @{thm sameShape1_def} @{thm F.mr_rel_map(1)}
-    @{thm F.mr_rel_map(2)} @{thm F.mr_rel_map(3)} @{thm F.map_comp} @{thm F.rel_eq} @{thm F.mr_rel_id} @{thm rel_F_exchange} 
-    @{thm F.mr_rel_flip} @{thm F.mr_rel_mono_strong0} @{thm F.mr_rel_Grp} @{context} 
-    THEN print_tac @{context} "done" THEN no_tac\<close>)*)
   subgoal premises prems
     apply (unfold nonrep2_def sameShape1_def)
     apply (rule allI)
     apply (rule impI)
     apply (erule exE)
+    apply (erule exE) (*repeat for each lin_pos*)
     apply (frule F.mr_rel_map(2)[rotated -1]; (rule prems supp_id_bound bij_id)?)
     apply (rotate_tac)
     apply (subst (asm) (1 2) trans[OF o_id id_o[symmetric]]) (*1..nr_non_lives*)
-    apply (subst (asm) (1) Grp_UNIV_id) (*lin_live_pos*)
+    apply (subst (asm) (1 3) Grp_UNIV_id) (*lin_live_pos*)
     apply (unfold trans[OF eq_OO OO_eq[symmetric]])
-    apply (subst (asm) (1) trans[OF OO_eq eq_OO[symmetric]]) (*lin_live_pos*)
-    apply (subst (asm) (1) eq_alt) (*lin_live_pos*)
+    apply (subst (asm) (1 3) trans[OF OO_eq eq_OO[symmetric]]) (*lin_live_pos*)
+    apply (subst (asm) (1 3) eq_alt) (*lin_live_pos*)
     apply (subst (asm) F.mr_rel_map(1)[symmetric]; (rule prems supp_id_bound bij_id)?)
     apply (insert prems(3)[unfolded nonrep2_def sameShape1_def]) (*lastprem*)
     apply (elim allE impE)
      apply (rule exI)
+     apply (rule exI)
      apply (assumption)
 
     apply (erule thin_rl)
+    apply (erule exE)
     apply (erule exE)
     apply (subst (asm) F.map_comp; (rule prems supp_id_bound bij_id)?)
     apply (unfold o_id id_o)
@@ -497,84 +270,30 @@ lemma nonrep2_map_F_rev:
      apply (rule iffD1[OF F.mr_rel_flip]; (rule supp_id_bound bij_id)?)
     apply (unfold inv_id)
     apply (subst (asm) F.mr_rel_map(3); (rule prems supp_id_bound bij_id)?)
-    apply (subst (asm) (1 2 3 4) Grp_def) (*TWICE for all lives *)
+    apply (subst (asm) (1 2 3 4 5 6) Grp_def) (*TWICE for all lives *)
     apply (subst (asm) (1 2) inv_o_simp1; (rule prems bij_id)?) (*for all frees and bounds*)
      apply (tactic \<open>unfold_thms_tac @{context} @{thms eqTrueI[OF UNIV_I] simp_thms(21) id_apply}\<close>) (*for all frees*)
-     apply (subst (asm) (1) eq_commute) (*lin_live_pos*)
+     apply (subst (asm) (1 5) eq_commute) (*some function of lin_live_pos*)
      apply (unfold eq_OO conversep_def)
-     apply (elim F.mr_rel_mono_strong0[rotated -5]; (rule supp_id_bound bij_id)?) (*- len vartypes - 1*)
+     apply (elim F.mr_rel_mono_strong0[rotated -6]; (rule supp_id_bound bij_id)?) (*- len vartypes - 1*)
       (*left subtactic is for frees and bounds, right subtactic for lives*)
     apply ((rule ballI,rule refl)?; (rule ballI,rule ballI,rule impI,rotate_tac 2,subst (asm) eq_commute,assumption))+
 
     apply (erule thin_rl)
-    apply (subst (asm) (1) Grp_UNIV_def[symmetric]) (*lin_live_pos*)
+    apply (subst (asm) (1 4) Grp_UNIV_def[symmetric]) (*some function of lin_live_pos*)
     apply (rule exI)
-    apply (subst (asm) (1) eq_alt) (* repeat lives - 1 *)
+    apply (rule exI) (*repeat for each lin_pos*)
+    apply (subst (asm) (1) eq_alt) (* repeat lives - (nr lin_poses) *)
     apply (subst (asm) F.mr_rel_Grp; (rule supp_id_bound bij_id)?)
     apply (unfold eqTrueI[OF subset_UNIV] eqTrueI[OF UNIV_I] UNIV_def[THEN sym] simp_thms(21) Grp_def)
     apply (assumption)
     done
   done
 
-ML\<open>
-open BNF_Util BNF_Tactics
-fun mk_nonrep2_map_bij_tac mrbnf nonrep_def sameShape_def F_mr_rel_map1 F_mr_rel_map3 F_map_id F_map_comp ctxt = 
-  HEADGOAL (Subgoal.FOCUS 
-    (fn {prems, context = ctxt, ...} => 
-      let
-        val id_prems = MRBNF_Comp_Tactics.mk_id_prems mrbnf;
-        val id_prems_v = MRBNF_Comp_Tactics.mk_prems mrbnf @{thms bij_id supp_id_bound} @{thms bij_id supp_id_bound}
-        val var_types = var_types_of_mrbnf mrbnf;
-        val nr_lives = length (filter (fn v => v = MRBNF_Def.Live_Var) var_types);
-        val lin_live_pos = fold_index (fn (i, v) => fn b => 
-          if (v = MRBNF_Def.Live_Var andalso i+1 < lin_pos) then b+1 else b) var_types 1;
-        val o_id_poses = map_range (fn i => if i < lin_pos-1 then i*2 + 7 else (i+1)*2 + 7) (length var_types-1) |> filter (fn n => n >= 0);
-      in
-        unfold_thms_tac ctxt [nonrep_def, sameShape_def] THEN
-        HEADGOAL (EVERY' [
-          rtac ctxt allI,
-          rtac ctxt impI,
-          etac ctxt exE,
-          dtac ctxt (rotate_prems ~1 (F_mr_rel_map1 RS iffD1)) THEN_ALL_NEW
-            TRY o resolve_tac ctxt @{thms bij_id supp_id_bound},
-          K (unfold_thms_tac ctxt @{thms o_id Grp_UNIV_id}),
-          EqSubst.eqsubst_asm_tac ctxt [lin_live_pos*3 - 1] [@{thm OO_eq} RS sym],
-          EqSubst.eqsubst_asm_tac ctxt (map_range (fn i => i+1) (nr_lives*2 -1)) [@{thm conversep_eq} RS sym],
-          EqSubst.eqsubst_asm_tac ctxt (map_range (fn i => i+1) (nr_lives*2 -1)) @{thms eq_alt},
-          EqSubst.eqsubst_asm_tac ctxt [1] [@{thm inv_o_simp2} OF [(nth prems 0)] RS sym],
-          K (unfold_thms_tac ctxt @{thms Grp_o converse_relcompp}),
-          EqSubst.eqsubst_asm_tac ctxt [1] [@{thm relcompp_assoc} RS sym],
-          dtac ctxt ((unfold_thms ctxt @{thms inv_id o_id} (F_mr_rel_map3 OF 
-            (id_prems @ id_prems_v) RS sym)) RS iffD1),
-          K (unfold_thms_tac ctxt @{thms Grp_UNIV_id conversep_eq}),
-          dtac ctxt (Object_Logic.rulify ctxt (unfold_thms ctxt [nonrep_def, sameShape_def] (nth prems 1)) OF [exI]),
-          etac ctxt exE
-        ]) THEN
-        HEADGOAL (Subgoal.FOCUS 
-          (fn {prems = subprems, context = ctxt, ...} => 
-            HEADGOAL (EVERY' [
-              EqSubst.eqsubst_tac ctxt [0] [F_map_id RS sym],
-              EqSubst.eqsubst_tac ctxt o_id_poses [@{thm o_id} RS sym],
-              EqSubst.eqsubst_tac ctxt [1] [@{thm inv_o_simp2} OF [(nth prems 0)] RS sym],
-              K (unfold_thms_tac ctxt [F_map_comp OF flat (replicate 2 id_prems) RS sym]),
-              EqSubst.eqsubst_tac ctxt [1] subprems,
-              EqSubst.eqsubst_tac ctxt [2*lin_pos + 6 + 2*(length var_types)] [@{thm o_id} RS sym],
-              EqSubst.eqsubst_tac ctxt [1] [@{thm inv_o_simp1} OF [(nth prems 0)] RS sym],
-              K (unfold_thms_tac ctxt [F_map_comp OF flat (replicate 2 id_prems)]),
-              EqSubst.eqsubst_tac ctxt [1, 2] @{thms o_assoc},
-              rtac ctxt exI,
-              rtac ctxt refl
-            ])
-          ) ctxt)
-      end)
-  ctxt)
-\<close>
-
-
 lemma nonrep2_mapF_bij:
-  fixes x :: "('a1::var,'a2::var,'a3,'a4) F" and g::"'a3\<Rightarrow>'a3"
-  assumes g: "bij g" and x: "nonrep2 x"
-  shows "nonrep2 (map_F id id g id x)" (is "nonrep2 ?x'")
+  fixes x :: "('a1::var,'a2::var,'a3,'a4,'a5) F" and g1 :: "'a3\<Rightarrow>'a3" and g2 :: "'a5\<Rightarrow>'a5" 
+  assumes "bij g1" "bij g2" and x: "nonrep2 x"
+  shows "nonrep2 (map_F id id g1 id g2 x)" (is "nonrep2 ?x'")
   using assms apply -
 (*  apply (tactic \<open>mk_nonrep2_map_bij_tac (MRBNF_Def.mrbnf_of @{context} @{type_name F} |> the) @{thm nonrep2_def}
     @{thm sameShape1_def} @{thm F.mr_rel_map(1)} @{thm F.mr_rel_map(3)} @{thm F.map_id} @{thm F.map_comp} @{context}
@@ -584,85 +303,75 @@ lemma nonrep2_mapF_bij:
     apply (rule allI)
     apply (rule impI)
     apply (erule exE)
+    apply (erule exE) (*repeat for each lin_pos*)
     apply (drule F.mr_rel_map(1)[THEN iffD1, rotated -1]; (rule supp_id_bound bij_id)?)
     apply (unfold o_id Grp_UNIV_id)
-    apply (subst (asm) (2) OO_eq[symmetric]) (*lin_live_pos * 3 - 1*)
-    apply (subst (asm) (1 2 3) conversep_eq[symmetric]) (* every pos (nr_lives * 2 - 1) *)
-    apply (subst (asm) (1 2 3) eq_alt) (* every pos (nr_lives * 2 - 1) *)
-    apply (subst (asm) (1) inv_o_simp2[OF g, symmetric]) (* second to last prem *)
+    apply (subst (asm) (2 9) OO_eq[symmetric]) (*lin_live_pos * 3 - 1 (needs to be adjusted)*)
+    apply (subst (asm) (1 2 3 4) conversep_eq[symmetric]) (* every pos (nr_lives * 2 - 1) *)
+    apply (subst (asm) (1 2 3 4) eq_alt) (* every pos (nr_lives * 2 - 1) *)
+    apply (subst (asm) (1) inv_o_simp2[OF prems(1), symmetric]) (* second to last prem *)
+    apply (subst (asm) (1) inv_o_simp2[OF prems(2), symmetric]) (*repeat for each lin_pos*)
     apply (unfold Grp_o converse_relcompp)
-    apply (subst (asm) (1) relcompp_assoc[symmetric]) (* 1 should be fine here, there should only be one chain of OO *)
-    apply (drule F.mr_rel_map(3)[THEN iffD2, OF supp_id_bound bij_id supp_id_bound bij_id
+    apply (subst (asm) (1 2) relcompp_assoc[symmetric]) (*repeat for each lin_pos*)
+    apply (drule F.mr_rel_map(3)[THEN iffD2, OF supp_id_bound bij_id supp_id_bound bij_id 
           supp_id_bound bij_id supp_id_bound, unfolded inv_id o_id])  (*bij and supp for bounds only supp for frees; THEN bij and supp for both *)
     apply (unfold Grp_UNIV_id conversep_eq)
-    apply (drule x[unfolded nonrep2_def sameShape1_def, rule_format, OF exI])
+    apply (drule prems(3)[unfolded nonrep2_def sameShape1_def, rule_format, OF exI, OF exI]) (*", OF exI" for each lin_pos*)
     apply (erule exE)
-    subgoal premises subprems for y' R' f
+    apply (erule exE) (*repeat for each lin_pos*)
+    subgoal premises subprems for y' R1' R2' f1 f2
       apply (subst (1) F.map_id[symmetric]) (*1 constant*)
-      apply (subst (7 9 13) o_id[symmetric]) (*target nth id by 2n + 7 starting at n=0  for all idx but lin_pos*)
-      apply (subst (1) inv_o_simp2[OF g, symmetric]) (*1 constant*)
-      apply (subst (1) F.map_comp[symmetric]; (rule bij_id supp_id_bound)?) (*1 constant*)
+      apply (subst (9 11 15) o_id[symmetric]) (*target nth id by <some function> starting at n=0 for all idx but lin_pos*)
+      apply (subst (1) inv_o_simp2[OF prems(1), symmetric])
+      apply (subst (1) inv_o_simp2[OF prems(2), symmetric]) (*repeat for each lin_pos*)
+      apply (subst (1) F.map_comp[symmetric]; (rule bij_id supp_id_bound)?)
       apply (subst (1) subprems) (*1 constant*)
-      apply (subst (20) o_id[symmetric]) (*target nth id by 2n + 6 + 2*nr vars starting at n=1  only for lin_pos*)
-      apply (subst (1) inv_o_simp1[OF g, symmetric]) (*1 constant*)
+      apply (subst (24 28) o_id[symmetric]) (*target nth id by <some function> starting at n=1 only for lin_pos*)
+      apply (subst (1) inv_o_simp1[OF prems(1), symmetric])
+      apply (subst (1) inv_o_simp1[OF prems(2), symmetric]) (*repeat for each lin_pos*)
       apply (subst (1 2) F.map_comp; (rule bij_id supp_id_bound)?) (*1 2 constant*)
-      apply (subst (1 2) o_assoc) (*1 2 constant*)
+      apply (subst (1 2 3 4) o_assoc) (*1 2 constant - 2 times for each lin_pos*)
+      apply (rule exI)
       apply (rule exI)
       apply (rule refl)
       done
     done
   done
 
-ML \<open>
-open BNF_Util BNF_Tactics
-
-fun mk_nonrep2_mapF_bij_2_tac mrbnf nonrep2_mapF_bij nonrep2_map_F F_map_comp ctxt =
-  HEADGOAL (Subgoal.FOCUS
-    (fn {prems, context = ctxt, ...} => 
-    let val nr_prems = length prems;
-        val id_prems = MRBNF_Comp_Tactics.mk_id_prems mrbnf;
-    in
-      HEADGOAL (rtac ctxt (unfold_thms ctxt ((F_map_comp OF ((take (nr_prems-2) prems) @ id_prems)) :: @{thms id_o o_id}) 
-        (nonrep2_mapF_bij OF [nth prems (nr_prems-2), nonrep2_map_F OF (nth_drop (nr_prems-2) prems)])
-      ))
-     end) ctxt)
-\<close>
-
 lemma nonrep2_mapF_bij_2:
-  fixes x :: "('a1::var,'a2::var,'a3,'a4) F"
-    and v :: "'a1 \<Rightarrow> 'a1" and u :: "'a2\<Rightarrow>'a2" and g::"'a3\<Rightarrow>'a3" and f::"'a4\<Rightarrow>'a4'"
+  fixes x :: "('a1::var,'a2::var,'a3,'a4,'a5) F"
+    and v :: "'a1 \<Rightarrow> 'a1" and u :: "'a2\<Rightarrow>'a2" and g1::"'a3\<Rightarrow>'a3" and f::"'a4\<Rightarrow>'a4'" and g2::"'a5\<Rightarrow>'a5" 
   assumes v: "|supp v| <o |UNIV :: 'a1 set|" and u: "bij u" "|supp u| <o |UNIV :: 'a2 set|"
-    and g: "bij g" and x: "nonrep2 x"
-  shows "nonrep2 (map_F v u g f x)" 
+    and "bij g1" "bij g2" and x: "nonrep2 x"
+  shows "nonrep2 (map_F v u g1 f g2 x)" 
   using assms apply -
-  apply (tactic \<open>mk_nonrep2_mapF_bij_2_tac (MRBNF_Def.mrbnf_of @{context} @{type_name F} |> the) 
-    @{thm nonrep2_mapF_bij} @{thm nonrep2_map_F} @{thm F.map_comp} @{context} 
-    THEN print_tac @{context} "done" THEN no_tac\<close>)
   subgoal premises prems
-    apply (rule nonrep2_mapF_bij[OF prems(4) nonrep2_map_F[OF prems(1,2,3,5)], 
+    apply (rule nonrep2_mapF_bij[OF prems(4,5) nonrep2_map_F[OF prems(1,2,3,6)], 
           unfolded F.map_comp[OF prems(1,2,3) supp_id_bound bij_id supp_id_bound] id_o o_id])
     done
   done
 
 
-typedef ('a1::var,'a2::var,'a3::var,'a4) F' = "{x :: ('a1,'a2,'a3,'a4) F. nonrep2 x}"
+typedef ('a1::var,'a2::var,'a3::var,'a4,'a5::var) F' = "{x :: ('a1,'a2,'a3,'a4,'a5) F. nonrep2 x}"
   apply (unfold mem_Collect_eq nonrep2_def sameShape1_def mr_rel_F_def F.map_id)
   by (rule ex_nonrep)
 
-definition set1_F' :: "('a1::var,'a2::var,'a3::var,'a4) F' \<Rightarrow> 'a1 set" where "set1_F' = set1_F o Rep_F'"
-definition set2_F' :: "('a1::var,'a2::var,'a3::var,'a4) F' \<Rightarrow> 'a2 set" where "set2_F' = set2_F o Rep_F'"
-definition set3_F' :: "('a1::var,'a2::var,'a3::var,'a4) F' \<Rightarrow> 'a3 set" where "set3_F' = set3_F o Rep_F'"
-definition set4_F' :: "('a1::var,'a2::var,'a3::var,'a4) F' \<Rightarrow> 'a4 set" where "set4_F' = set4_F o Rep_F'"
+definition set1_F' :: "('a1::var,'a2::var,'a3::var,'a4,'a5::var) F' \<Rightarrow> 'a1 set" where "set1_F' = set1_F o Rep_F'"
+definition set2_F' :: "('a1::var,'a2::var,'a3::var,'a4,'a5::var) F' \<Rightarrow> 'a2 set" where "set2_F' = set2_F o Rep_F'"
+definition set3_F' :: "('a1::var,'a2::var,'a3::var,'a4,'a5::var) F' \<Rightarrow> 'a3 set" where "set3_F' = set3_F o Rep_F'"
+definition set4_F' :: "('a1::var,'a2::var,'a3::var,'a4,'a5::var) F' \<Rightarrow> 'a4 set" where "set4_F' = set4_F o Rep_F'"
+definition set5_F' :: "('a1::var,'a2::var,'a3::var,'a4,'a5::var) F' \<Rightarrow> 'a5 set" where "set5_F' = set5_F o Rep_F'"
 
 definition asSS :: "('a \<Rightarrow> 'a) \<Rightarrow> 'a \<Rightarrow> 'a" where
   "asSS f \<equiv> if |supp f| <o |UNIV :: 'a set| then f else id"
 
 definition map_F' :: "('a1::var \<Rightarrow> 'a1) \<Rightarrow> ('a2::var \<Rightarrow> 'a2) \<Rightarrow> ('a3::var \<Rightarrow> 'a3) \<Rightarrow> ('a4 \<Rightarrow> 'a4') 
-  \<Rightarrow> ('a1,'a2,'a3,'a4) F' \<Rightarrow> ('a1,'a2,'a3,'a4') F'"
-  where "map_F' v u f g = Abs_F' o map_F (asSS v) (asSS (asBij u)) (asBij f) g o Rep_F'"
+  \<Rightarrow> ('a5::var \<Rightarrow> 'a5)  
+  \<Rightarrow> ('a1,'a2,'a3,'a4,'a5) F' \<Rightarrow> ('a1,'a2,'a3,'a4','a5) F'"
+  where "map_F' v u f1 g f2 = Abs_F' o map_F (asSS v) (asSS (asBij u)) (asBij f1) g (asBij f2) o Rep_F'"
 
-definition rrel_F' :: "('a4 \<Rightarrow> 'a4' \<Rightarrow> bool) \<Rightarrow> ('a1::var,'a2::var,'a3::var,'a4) F' \<Rightarrow> ('a1,'a2,'a3,'a4') F' \<Rightarrow> bool"
-  where "rrel_F' R x x' = rrel_F (=) R (Rep_F' x) (Rep_F' x')"
+definition rrel_F' :: "('a4 \<Rightarrow> 'a4' \<Rightarrow> bool) \<Rightarrow> ('a1::var,'a2::var,'a3::var,'a4,'a5::var) F' \<Rightarrow> ('a1,'a2,'a3,'a4','a5) F' \<Rightarrow> bool"
+  where "rrel_F' R x x' = rrel_F (=) R (=) (Rep_F' x) (Rep_F' x')"
 
 (* Verifying the axioms of a MRBNF for F':  *)
 ML \<open>
@@ -681,22 +390,17 @@ fun mk_map_id_tac map_F'_def F_map_id Rep_F'_inverse ctxt =
      ) ctxt)
 \<close>
 
-lemma F'_map_id: "map_F' id id id id = id"
-  apply (tactic \<open>mk_map_id_tac @{thm map_F'_def} @{thm F.map_id} @{thm Rep_F'_inverse} @{context} 
-    THEN print_tac @{context} "done" THEN no_tac\<close>)
-  apply (unfold map_F'_def asSS_def asBij_def 
-      eqTrueI[OF bij_id] eqTrueI[OF supp_id_bound] if_True)
-  apply (rule ext)
-  apply (unfold o_apply F.map_id Rep_F'_inverse)
-  apply (unfold id_def)
-  apply (rule refl)
-  done
+lemma F'_map_id: "map_F' id id id id id = id"
+  by (tactic \<open>mk_map_id_tac @{thm map_F'_def} @{thm F.map_id} @{thm Rep_F'_inverse} @{context} 
+    THEN print_tac @{context} "done"\<close>)
 
 
 ML \<open>
 open BNF_Util BNF_Tactics
 
 fun mk_map_comp_tac mrbnf map_F'_def Abs_F'_inverse Rep_F' nonrep2_mapF_bij_2 F_map_comp0 ctxt =
+
+  (* For this only the second "apply" needs to be adjusted: (length lin_poses instead of "1")*)
   HEADGOAL (Subgoal.FOCUS
     (fn {prems = prems, context = ctxt, ...} =>
     let
@@ -705,7 +409,7 @@ fun mk_map_comp_tac mrbnf map_F'_def Abs_F'_inverse Rep_F' nonrep2_mapF_bij_2 F_
       val nr_frees = length (filter (fn v => v = MRBNF_Def.Free_Var) var_types);
     in
       unfold_thms_tac ctxt (map_F'_def:: @{thms asSS_def asBij_def}) THEN
-      HEADGOAL(EqSubst.eqsubst_tac ctxt (map_range (fn i => i+1) (1 + 2*nr_bounds)) @{thms bij_comp} THEN_ALL_NEW
+      HEADGOAL(EqSubst.eqsubst_tac ctxt (map_range (fn i => i+1) (length lin_poses + 2*nr_bounds)) @{thms bij_comp} THEN_ALL_NEW
         TRY o resolve_tac ctxt prems) THEN
       unfold_thms_tac ctxt @{thms if_True} THEN
       HEADGOAL (EqSubst.eqsubst_tac ctxt (map_range (fn i => i+1) (nr_bounds + nr_frees)) @{thms supp_comp_bound} THEN_ALL_NEW
@@ -721,28 +425,31 @@ fun mk_map_comp_tac mrbnf map_F'_def Abs_F'_inverse Rep_F' nonrep2_mapF_bij_2 F_
     end) ctxt)
 \<close>
 
+(* For this only the second "apply" needs to be adjusted: (length lin_poses instead of "1")*)
 lemma F'_map_comp1_:
   fixes u1 v1 :: "'a1::var \<Rightarrow> 'a1"
   fixes u2 v2 :: "'a2::var \<Rightarrow> 'a2"
   fixes u3 v3 :: "'a3::var \<Rightarrow> 'a3"
+  fixes u5 v5 :: "'a5::var \<Rightarrow> 'a5"
   assumes "|supp u1| <o |UNIV :: 'a1 set|" "|supp v1| <o |UNIV :: 'a1 set|"
   assumes "bij u2" "|supp u2| <o |UNIV :: 'a2 set|" "bij v2" "|supp v2| <o |UNIV :: 'a2 set|"
   assumes "bij u3" "|supp u3| <o |UNIV :: 'a3 set|" "bij v3" "|supp v3| <o |UNIV :: 'a3 set|"
-  shows "map_F' (v1 o u1) (v2 o u2) (v3 o u3) (g o f) = map_F' v1 v2 v3 g o map_F' u1 u2 u3 f"
+  assumes "bij u5" "|supp u5| <o |UNIV :: 'a5 set|" "bij v5" "|supp v5| <o |UNIV :: 'a5 set|"
+  shows "map_F' (v1 o u1) (v2 o u2) (v3 o u3) (g o f) (v5 o u5) = map_F' v1 v2 v3 g v5 o map_F' u1 u2 u3 f u5"
   using assms apply -
-  apply (tactic \<open>mk_map_comp_tac (MRBNF_Def.mrbnf_of @{context} @{type_name F} |> the) @{thm map_F'_def} 
-    @{thm Abs_F'_inverse[unfolded mem_Collect_eq]} @{thm Rep_F'[unfolded mem_Collect_eq]} @{thm nonrep2_mapF_bij_2}
-     @{thm F.map_comp0} @{context} 
+  apply (tactic \<open>mk_map_comp_tac (MRBNF_Def.mrbnf_of @{context} @{type_name F} |> the) @{thm map_F'_def} @{thm Abs_F'_inverse[unfolded mem_Collect_eq]}
+    @{thm Rep_F'[unfolded mem_Collect_eq]} @{thm nonrep2_mapF_bij_2} @{thm F.map_comp0} @{context} 
     THEN print_tac @{context} "done" THEN no_tac\<close>)
   subgoal premises prems
     apply (unfold map_F'_def asBij_def asSS_def)
-    apply (subst (1 2 3) bij_comp; (rule prems)?) (* 1(lin) + 2*bounds *)
+    apply (subst (1 2 3 4) bij_comp; (rule prems)?) (* 1*(lin_poses) + 2*bounds *)
     apply (unfold if_True)
     apply (subst (1 2) supp_comp_bound; (rule prems infinite_UNIV)?) (* bounds + frees *)
     apply (unfold if_True)
     apply (unfold 
         eqTrueI[OF assms(1)] eqTrueI[OF assms(2)] eqTrueI[OF assms(3)] eqTrueI[OF assms(4)] eqTrueI[OF assms(5)] eqTrueI[OF assms(6)]
-        eqTrueI[OF assms(7)] eqTrueI[OF assms(8)] eqTrueI[OF assms(9)] eqTrueI[OF assms(10)]
+        eqTrueI[OF assms(7)] eqTrueI[OF assms(8)] eqTrueI[OF assms(9)] eqTrueI[OF assms(10)] eqTrueI[OF assms(11)] 
+        eqTrueI[OF assms(12)] eqTrueI[OF assms(13)] eqTrueI[OF assms(14)]
         if_True)
     apply (rule ext)
     apply (subst F.map_comp0; (rule prems)?)
@@ -775,62 +482,76 @@ lemma F'_set1_map_:
   fixes u1 :: "'a1::var \<Rightarrow> 'a1"
   fixes u2 :: "'a2::var \<Rightarrow> 'a2"
   fixes u3 :: "'a3::var \<Rightarrow> 'a3"
+  fixes u5 :: "'a5::var \<Rightarrow> 'a5"
   assumes "|supp u1| <o |UNIV :: 'a1 set|"
   assumes "bij u2" "|supp u2| <o |UNIV :: 'a2 set|"
   assumes "bij u3" "|supp u3| <o |UNIV :: 'a3 set|"
-  shows "set1_F' (map_F' u1 u2 u3 f b) = u1 ` set1_F' b"
+  assumes "bij u5" "|supp u5| <o |UNIV :: 'a5 set|"
+  shows "set1_F' (map_F' u1 u2 u3 f u5 b) = u1 ` set1_F' b"
   using assms apply -
-  apply (tactic \<open>mk_set_map_tac @{thm set1_F'_def} @{thm map_F'_def} @{thm Abs_F'_inverse[unfolded mem_Collect_eq]}
+  by (tactic \<open>mk_set_map_tac @{thm set1_F'_def} @{thm map_F'_def} @{thm Abs_F'_inverse[unfolded mem_Collect_eq]}
     @{thm Rep_F'[unfolded mem_Collect_eq]} @{thm nonrep2_mapF_bij_2} @{thm F.set_map(1)} @{context} 
-    THEN print_tac @{context} "done" THEN no_tac\<close>)
-  subgoal premises prems
-    apply (unfold set1_F'_def map_F'_def asSS_def asBij_def
-        eqTrueI[OF prems(1)] eqTrueI[OF prems(2)] eqTrueI[OF prems(3)] eqTrueI[OF prems(4)] eqTrueI[OF prems(5)] o_apply if_True)
-    apply (subst Abs_F'_inverse[unfolded mem_Collect_eq])
-     apply (rule nonrep2_mapF_bij_2; (rule prems Rep_F'[unfolded mem_Collect_eq])?)
-    apply (rule F.set_map(1); (rule prems))
-    done
-  done
+    THEN print_tac @{context} "done"\<close>)
 
 lemma F'_set2_map_:
   fixes u1 :: "'a1::var \<Rightarrow> 'a1"
   fixes u2 :: "'a2::var \<Rightarrow> 'a2"
   fixes u3 :: "'a3::var \<Rightarrow> 'a3"
+  fixes u5 :: "'a5::var \<Rightarrow> 'a5"
   assumes "|supp u1| <o |UNIV :: 'a1 set|"
   assumes "bij u2" "|supp u2| <o |UNIV :: 'a2 set|"
   assumes "bij u3" "|supp u3| <o |UNIV :: 'a3 set|"
-  shows "set2_F' (map_F' u1 u2 u3 f b) = u2 ` set2_F' b"
+  assumes "bij u5" "|supp u5| <o |UNIV :: 'a5 set|"
+  shows "set2_F' (map_F' u1 u2 u3 f u5 b) = u2 ` set2_F' b"
   using assms apply -
-  apply (tactic \<open>mk_set_map_tac @{thm set2_F'_def} @{thm map_F'_def} @{thm Abs_F'_inverse[unfolded mem_Collect_eq]}
-    @{thm Rep_F'[unfolded mem_Collect_eq]} @{thm nonrep2_mapF_bij_2} @{thm F.set_map(2)} @{context}\<close>)
-  done
+  by (tactic \<open>mk_set_map_tac @{thm set2_F'_def} @{thm map_F'_def} @{thm Abs_F'_inverse[unfolded mem_Collect_eq]}
+    @{thm Rep_F'[unfolded mem_Collect_eq]} @{thm nonrep2_mapF_bij_2} @{thm F.set_map(2)} @{context} 
+    THEN print_tac @{context} "done"\<close>)
 
 lemma F'_set3_map_:
   fixes u1 :: "'a1::var \<Rightarrow> 'a1"
   fixes u2 :: "'a2::var \<Rightarrow> 'a2"
   fixes u3 :: "'a3::var \<Rightarrow> 'a3"
+  fixes u5 :: "'a5::var \<Rightarrow> 'a5"
   assumes "|supp u1| <o |UNIV :: 'a1 set|"
   assumes "bij u2" "|supp u2| <o |UNIV :: 'a2 set|"
   assumes "bij u3" "|supp u3| <o |UNIV :: 'a3 set|"
-  shows "set3_F' (map_F' u1 u2 u3 f b) = u3 ` set3_F' b"
+  assumes "bij u5" "|supp u5| <o |UNIV :: 'a5 set|"
+  shows "set3_F' (map_F' u1 u2 u3 f u5 b) = u3 ` set3_F' b"
   using assms apply -
-  apply (tactic \<open>mk_set_map_tac @{thm set3_F'_def} @{thm map_F'_def} @{thm Abs_F'_inverse[unfolded mem_Collect_eq]}
-    @{thm Rep_F'[unfolded mem_Collect_eq]} @{thm nonrep2_mapF_bij_2} @{thm F.set_map(3)} @{context}\<close>)
-  done
+  by (tactic \<open>mk_set_map_tac @{thm set3_F'_def} @{thm map_F'_def} @{thm Abs_F'_inverse[unfolded mem_Collect_eq]}
+    @{thm Rep_F'[unfolded mem_Collect_eq]} @{thm nonrep2_mapF_bij_2} @{thm F.set_map(3)} @{context} 
+    THEN print_tac @{context} "done"\<close>)
 
 lemma F'_set4_map_:
   fixes u1 :: "'a1::var \<Rightarrow> 'a1"
   fixes u2 :: "'a2::var \<Rightarrow> 'a2"
   fixes u3 :: "'a3::var \<Rightarrow> 'a3"
+  fixes u5 :: "'a5::var \<Rightarrow> 'a5"
   assumes "|supp u1| <o |UNIV :: 'a1 set|"
   assumes "bij u2" "|supp u2| <o |UNIV :: 'a2 set|"
   assumes "bij u3" "|supp u3| <o |UNIV :: 'a3 set|"
-  shows "set4_F' (map_F' u1 u2 u3 f b) = f ` set4_F' b"
+  assumes "bij u5" "|supp u5| <o |UNIV :: 'a5 set|"
+  shows "set4_F' (map_F' u1 u2 u3 f u5 b) = f ` set4_F' b"
   using assms apply -
-  apply (tactic \<open>mk_set_map_tac @{thm set4_F'_def} @{thm map_F'_def} @{thm Abs_F'_inverse[unfolded mem_Collect_eq]}
-    @{thm Rep_F'[unfolded mem_Collect_eq]} @{thm nonrep2_mapF_bij_2} @{thm F.set_map(4)} @{context}\<close>)
-  done
+  by (tactic \<open>mk_set_map_tac @{thm set4_F'_def} @{thm map_F'_def} @{thm Abs_F'_inverse[unfolded mem_Collect_eq]}
+    @{thm Rep_F'[unfolded mem_Collect_eq]} @{thm nonrep2_mapF_bij_2} @{thm F.set_map(4)} @{context} 
+    THEN print_tac @{context} "done"\<close>)
 
+lemma F'_set5_map_:
+  fixes u1 :: "'a1::var \<Rightarrow> 'a1"
+  fixes u2 :: "'a2::var \<Rightarrow> 'a2"
+  fixes u3 :: "'a3::var \<Rightarrow> 'a3"
+  fixes u5 :: "'a5::var \<Rightarrow> 'a5"
+  assumes "|supp u1| <o |UNIV :: 'a1 set|"
+  assumes "bij u2" "|supp u2| <o |UNIV :: 'a2 set|"
+  assumes "bij u3" "|supp u3| <o |UNIV :: 'a3 set|"
+  assumes "bij u5" "|supp u5| <o |UNIV :: 'a5 set|"
+  shows "set5_F' (map_F' u1 u2 u3 f u5 b) = u5 ` set5_F' b"
+  using assms apply -
+  by (tactic \<open>mk_set_map_tac @{thm set5_F'_def} @{thm map_F'_def} @{thm Abs_F'_inverse[unfolded mem_Collect_eq]}
+    @{thm Rep_F'[unfolded mem_Collect_eq]} @{thm nonrep2_mapF_bij_2} @{thm F.set_map(5)} @{context} 
+    THEN print_tac @{context} "done"\<close>)
 
 ML \<open>
 open BNF_Util BNF_Tactics
@@ -854,38 +575,21 @@ lemma F'_map_cong_[fundef_cong]:
   fixes u1 v1 :: "'a1::var \<Rightarrow> 'a1"
   fixes u2 v2 :: "'a2::var \<Rightarrow> 'a2"
   fixes u3 v3 :: "'a3::var \<Rightarrow> 'a3"
+  fixes u5 v5 :: "'a5::var \<Rightarrow> 'a5"
   assumes "|supp u1| <o |UNIV :: 'a1 set|" "|supp v1| <o |UNIV :: 'a1 set|"
   assumes "bij u2" "|supp u2| <o |UNIV :: 'a2 set|" "bij v2" "|supp v2| <o |UNIV :: 'a2 set|"
   assumes "bij u3" "|supp u3| <o |UNIV :: 'a3 set|" "bij v3" "|supp v3| <o |UNIV :: 'a3 set|"
+  assumes "bij u5" "|supp u5| <o |UNIV :: 'a5 set|" "bij v5" "|supp v5| <o |UNIV :: 'a5 set|"
     and "\<forall> a \<in> set1_F' x. u1 a = v1 a"
     and "\<forall> a \<in> set2_F' x. u2 a = v2 a"
     and "\<forall> a \<in> set3_F' x. u3 a = v3 a"
     and "\<forall> a \<in> set4_F' x. f a = g a"
-  shows "map_F' u1 u2 u3 f x = map_F' v1 v2 v3 g x"
+    and "\<forall> a \<in> set5_F' x. u5 a = v5 a"
+  shows "map_F' u1 u2 u3 f u5 x = map_F' v1 v2 v3 g v5 x"
   using assms apply -
-  apply (tactic \<open>mk_map_cong_tac @{thm map_F'_def} @{thm F.map_cong} 
-    @{thms set1_F'_def set2_F'_def set3_F'_def set4_F'_def} @{context} 
-    THEN print_tac @{context} "done" THEN no_tac\<close>)
-  subgoal premises prems
-    apply (unfold map_F'_def asSS_def asBij_def 
-        eqTrueI[OF assms(1)] eqTrueI[OF assms(2)] eqTrueI[OF assms(3)] eqTrueI[OF assms(4)] eqTrueI[OF assms(5)] 
-        eqTrueI[OF assms(6)] eqTrueI[OF assms(7)] eqTrueI[OF assms(8)] eqTrueI[OF assms(9)] eqTrueI[OF assms(10)]
-        eqTrueI[OF assms(11)] eqTrueI[OF assms(12)] eqTrueI[OF assms(13)] eqTrueI[OF assms(14)] if_True o_apply)
-    apply (subst F.map_cong; (rule prems(14,13,12,11,10,9,8,7,6,5,4,3,2,1))?) (*reverse prems so that the v-prems apply before the u-prems*)
-         apply (rule refl)
-        apply (insert prems(11)[rule_format]) []
-        apply (drule ballI)
-(* \<And>z1. \<lbrakk>z1 \<in> set1_F (Rep_F'' xa); \<forall>z1\<in>set1_F (Rep_F'' xa). f1a z1 = g1a z1\<rbrakk> \<Longrightarrow> z1 \<in> set1_F (Rep_F'' xa) *)
-        apply (unfold set1_F'_def o_apply)
-        apply (erule bspec)
-    apply (assumption)
-         apply (erule bspec[OF prems(11)[unfolded set1_F'_def o_apply]] 
-        bspec[OF prems(12)[unfolded set2_F'_def o_apply]]
-        bspec[OF prems(13)[unfolded set3_F'_def o_apply]]
-        bspec[OF prems(14)[unfolded set4_F'_def o_apply]])+
-    apply (rule refl)
-    done
-  done
+  by (tactic \<open>mk_map_cong_tac @{thm map_F'_def} @{thm F.map_cong} 
+    @{thms set1_F'_def set2_F'_def set3_F'_def set4_F'_def set5_F'_def} @{context} 
+    THEN print_tac @{context} "done"\<close>)
 
 
 (* This tactic is applicable to all 4 of the following <F'_setx_bd> lemmas*)
@@ -898,20 +602,16 @@ fun mk_set_bd_tac set_F'_def F_set_bd ctxt =
 \<close>
 
 lemma F'_set1_bd: "\<And>b. |set1_F' b| <o natLeq"
-  apply (tactic \<open>mk_set_bd_tac @{thm set1_F'_def} @{thm F.set_bd(1)} @{context}
-    THEN print_tac @{context} "done" THEN no_tac\<close>)
-  apply (unfold set1_F'_def o_apply)
-  apply (rule F.set_bd(1))
-  done
+  by (tactic \<open>mk_set_bd_tac @{thm set1_F'_def} @{thm F.set_bd(1)} @{context}
+    THEN print_tac @{context} "done"\<close>)
 lemma F'_set2_bd: "\<And>b. |set2_F' b| <o natLeq"
-  apply (tactic \<open>mk_set_bd_tac @{thm set2_F'_def} @{thm F.set_bd(2)} @{context}\<close>)
-  done
+  by (tactic \<open>mk_set_bd_tac @{thm set2_F'_def} @{thm F.set_bd(2)} @{context}\<close>)
 lemma F'_set3_bd: "\<And>b. |set3_F' b| <o natLeq"
-  apply (tactic \<open>mk_set_bd_tac @{thm set3_F'_def} @{thm F.set_bd(3)} @{context}\<close>)
-  done
+  by (tactic \<open>mk_set_bd_tac @{thm set3_F'_def} @{thm F.set_bd(3)} @{context}\<close>)
 lemma F'_set4_bd: "\<And>b. |set4_F' b| <o natLeq"
-  apply (tactic \<open>mk_set_bd_tac @{thm set4_F'_def} @{thm F.set_bd(4)} @{context}\<close>)
-  done
+  by (tactic \<open>mk_set_bd_tac @{thm set4_F'_def} @{thm F.set_bd(4)} @{context}\<close>)
+lemma F'_set5_bd: "\<And>b. |set5_F' b| <o natLeq"
+  by (tactic \<open>mk_set_bd_tac @{thm set5_F'_def} @{thm F.set_bd(5)} @{context}\<close>)
 
 ML \<open>
 open BNF_Util BNF_Tactics
@@ -921,7 +621,7 @@ fun mk_rel_comp_leq_tac rrel_F'_def F_rel_compp ctxt =
     rtac ctxt @{thm predicate2I},
     etac ctxt @{thm relcomppE},
     K (unfold_thms_tac ctxt [rrel_F'_def]),
-    EqSubst.eqsubst_tac ctxt [1] (@{thms eq_OO[symmetric]}),
+    EqSubst.eqsubst_tac ctxt [1, 6] (@{thms eq_OO[symmetric]}),
     EqSubst.eqsubst_tac ctxt [1] ([F_rel_compp]),
     K (unfold_thms_tac ctxt [rrel_F'_def]),
     rtac ctxt @{thm relcomppI} THEN_ALL_NEW assume_tac ctxt
@@ -934,7 +634,7 @@ lemma F'_rel_comp_leq_: "rrel_F' Q OO rrel_F' R \<le> rrel_F' (Q OO R)"
   apply (rule predicate2I)
   apply (erule relcomppE)
   apply (unfold rrel_F'_def)
-  apply (subst (1) eq_OO[symmetric])
+  apply (subst (1 6) eq_OO[symmetric]) (* needs to be done for each lin_pos*)
   apply (subst (1) F.rel_compp)
   apply (rule relcomppI; (assumption))
   done
@@ -950,14 +650,10 @@ fun mk_rrel_F_map_F3_tac F_rel_map F_rel_mono_strong Grp_def ctxt =
 \<close>
 
 lemma rrel_F_map_F3:
-  fixes x :: "('a :: var,'b :: var,'c,'d) F"
-  shows "rrel_F (Grp (f :: 'c \<Rightarrow> 'c)) R x y = rrel_F (=) R (map_F id id f id x) y"
-  apply (tactic \<open>mk_rrel_F_map_F3_tac @{thm F.rel_map(1)} @{thm F.rel_mono_strong} @{thm Grp_def} @{context} 
-    THEN print_tac @{context} "done" THEN no_tac\<close>)
-  apply (unfold F.rel_map(1) Grp_def id_apply eqTrueI[OF UNIV_I] simp_thms(21))
-  apply (rule iffI)
-   apply (erule F.rel_mono_strong; (assumption?,(erule sym)?))+
-  done
+  fixes x :: "('a :: var,'b :: var,'c,'d,'e) F"
+  shows "rrel_F (Grp (f1 :: 'c \<Rightarrow> 'c)) R (Grp (f2 :: 'e \<Rightarrow> 'e)) x y = rrel_F (=) R (=) (map_F id id f1 id f2 x) y"
+  by (tactic \<open>mk_rrel_F_map_F3_tac @{thm F.rel_map(1)} @{thm F.rel_mono_strong} @{thm Grp_def} @{context} 
+    THEN print_tac @{context} "done"\<close>)
 
 
 ML \<open>
@@ -970,14 +666,8 @@ fun mk_asSS_tac ctxt =
 \<close>
 
 lemma asSS: "|supp u| <o |UNIV :: 'a set| \<Longrightarrow> asSS (u :: 'a \<Rightarrow> 'a) = u"
-  apply (tactic \<open>mk_asSS_tac @{context} 
-    THEN print_tac @{context} "done" THEN no_tac\<close>)
-  subgoal premises prems
-    apply (unfold asSS_def)
-    apply (rule if_P) 
-    apply (rule prems)
-    done
-  done
+  by (tactic \<open>mk_asSS_tac @{context} 
+    THEN print_tac @{context} "done"\<close>)
 
 ML \<open>
 open BNF_Util BNF_Tactics MRBNF_Def
@@ -1107,28 +797,24 @@ lemma F'_in_rel:
   fixes u1 :: "'a1::var \<Rightarrow> 'a1"
   fixes u2 :: "'a2::var \<Rightarrow> 'a2"
   fixes u3 :: "'a3::var \<Rightarrow> 'a3"
+  fixes u5 :: "'a5::var \<Rightarrow> 'a5"
   assumes u1: "|supp u1| <o |UNIV :: 'a1 set|"
     and u2: "bij u2" "|supp u2| <o |UNIV :: 'a2 set|" 
     and u3: "bij u3" "|supp u3| <o |UNIV :: 'a3 set|"
-  shows "rrel_F' R (map_F' u1 u2 u3 id x) y =
-    (\<exists>z. set4_F' z \<subseteq> {(x, y). R x y} \<and> map_F' id id id fst z = x \<and> map_F' u1 u2 u3 snd z = y)"
+    and u5: "bij u5" "|supp u5| <o |UNIV :: 'a5 set|"
+  shows "rrel_F' R (map_F' u1 u2 u3 id u5 x) y =
+    (\<exists>z. set4_F' z \<subseteq> {(x, y). R x y} \<and> map_F' id id id fst id z = x \<and> map_F' u1 u2 u3 snd u5 z = y)"
   using assms apply -
-  (*apply (tactic \<open>mk_in_rel_tac (MRBNF_Def.mrbnf_of @{context} @{type_name F} |> the) @{thm rrel_F'_def} 
-    @{thm map_F'_def} @{thm Abs_F'_inverse[unfolded mem_Collect_eq]}
-    @{thm Rep_F'[unfolded mem_Collect_eq]} @{thm nonrep2_mapF_bij_2} @{thm rrel_F_map_F3} @{thm F.in_rel}
-    @{thm F.map_comp} @{thm nonrep2_map_F_rev} @{thm Rep_F'_inverse} @{thm F.map_cong} @{thms set4_F'_def} @{thms F.set_map}
-    @{cterm x} @{context}
-    THEN print_tac @{context} "done" THEN no_tac\<close>)*)
   subgoal premises prems
     apply (unfold rrel_F'_def set4_F'_def map_F'_def asSS_def asBij_def if_True 
         eqTrueI[OF prems(1)] eqTrueI[OF prems(2)] eqTrueI[OF prems(3)] eqTrueI[OF prems(4)] 
-        eqTrueI[OF prems(5)]
+        eqTrueI[OF prems(5)] eqTrueI[OF prems(6)] eqTrueI[OF prems(7)]
         eqTrueI[OF supp_id_bound] eqTrueI[OF bij_id] o_apply)
     apply (subst Abs_F'_inverse[unfolded mem_Collect_eq])
      apply (rule nonrep2_mapF_bij_2; (rule prems Rep_F'[unfolded mem_Collect_eq])?)
 
-    apply (subst (11 13 15 17) id_o[THEN sym]) (* 2*nr_lives + 7*)
-    apply (subst (3) trans[OF id_o o_id[THEN sym]])
+    apply (subst (13 15 17 19 21) id_o[THEN sym]) (* 2*nr_lives + 7*)
+    apply (subst (3 5) trans[OF id_o o_id[THEN sym]])
     apply (subst F.map_comp[symmetric]; (rule prems bij_id supp_id_bound)?)
     apply (subst rrel_F_map_F3[symmetric])
     apply (subst F.in_rel; (rule prems)?)
@@ -1141,42 +827,16 @@ lemma F'_in_rel:
      apply (erule conjE)
      apply (erule CollectE)
      apply (erule conjE)
+     apply (erule conjE)
     subgoal premises subprems for z
-(*   apply (tactic \<open>
-        let
-          val ctxt = @{context};
-          val cz = @{cterm z};
-          val z = Thm.term_of cz;
-          val zT = fastype_of z;
-          val which = 0;
-          val Abs_F' = @{term Abs_F'}
-          val mrbnf = MRBNF_Def.mrbnf_of ctxt @{type_name F} |> the;
-          val subst = Sign.typ_match (Proof_Context.theory_of ctxt)
-            (MRBNF_Def.T_of_mrbnf mrbnf, zT) Vartab.empty |> @{print};
-          val deads = MRBNF_Def.deads_of_mrbnf mrbnf |> map (Envir.subst_type subst) |> @{print};
-          val frees = MRBNF_Def.frees_of_mrbnf mrbnf |> map (Envir.subst_type subst) |> @{print};
-          val bounds = MRBNF_Def.bounds_of_mrbnf mrbnf |> map (Envir.subst_type subst) |> @{print};
-          val lives = MRBNF_Def.lives_of_mrbnf mrbnf |> map (Envir.subst_type subst) |> @{print};
-          val map_F = MRBNF_Def.mk_map_comb_of_mrbnf deads
-            (map_index (uncurry (fn i => if i = which then BNF_Util.fst_const else HOLogic.id_const)) lives)
-            (map HOLogic.id_const bounds) (map HOLogic.id_const frees)
-            mrbnf $ z |> @{print};
-          val Ts = fastype_of map_F |> dest_Type |> snd;
-          val Us = domain_type (fastype_of Abs_F') |> dest_Type |> snd;
-          val ct = Thm.cterm_of ctxt (subst_atomic_types (Us ~~ Ts) Abs_F' $ map_F) |> @{print};
-        in
-          HEADGOAL (BNF_Util.rtac ctxt (infer_instantiate' ctxt [NONE, SOME ct] exI))
-        end
-        \<close>)*)
       apply (rule exI)
       apply (subst (1 2 3) Abs_F'_inverse[unfolded mem_Collect_eq])
        apply (insert Rep_F'[of x, unfolded mem_Collect_eq subprems(1)[symmetric]]) []
-       apply (subst (asm) (4 6 8 10) o_id[symmetric]) (*add o_id on all right sides*)
-       apply (subst (asm) (3) trans[OF o_id id_o[symmetric]])  (*move lin_pos to the left*)
+       apply (subst (asm) (4 6 8 10 12) o_id[symmetric]) (*add o_id on all right sides*)
+       apply (subst (asm) (3 5) trans[OF o_id id_o[symmetric]])  (*move lin_pos to the left*)
        apply (subst (asm) F.map_comp[symmetric]; (rule bij_id supp_id_bound)?)
        apply (drule nonrep2_map_F_rev[rotated -1]; (rule bij_id supp_id_bound)?)
        apply (assumption)
-
       apply (subst (1 2) F.map_comp; (rule supp_id_bound bij_id prems)?)
       apply (unfold o_id id_o)
       apply (rule conjI)
@@ -1189,6 +849,12 @@ lemma F'_in_rel:
        apply (rule arg_cong[OF subprems(1)])
       apply (subst subprems(2)[symmetric])
       apply (rule F.map_cong[THEN arg_cong]; (rule prems refl)?)
+      apply (drule rev_subsetD[THEN Collect_case_prodD])
+       apply (rule subprems)
+      apply (rule sym)
+      apply (subst o_apply)
+       apply (assumption)
+  (*repeat this block for each lin_pos*)
       apply (drule rev_subsetD[THEN Collect_case_prodD])
        apply (rule subprems)
       apply (rule sym)
@@ -1213,7 +879,7 @@ lemma F'_in_rel:
         apply (unfold o_id)
         apply (unfold o_def)
         apply (rule F.map_cong; (rule prems refl)?)
-        apply (rule snd_conv)
+        apply (rule snd_conv)+ (*repeat for each lin_pos*)
 
        apply (rule CollectI)
        apply (subst F.set_map; (rule bij_id supp_id_bound)?)+
@@ -1222,7 +888,19 @@ lemma F'_in_rel:
         apply (rule subsetI)
         apply (erule imageE)
         apply (rule CollectI)
-       apply (rule case_prodI2)
+        apply (rule case_prodI2)
+        apply (drule trans[OF sym, THEN iffD1[OF prod.inject]])
+         apply (assumption)
+        apply (erule conjE)
+        apply (rule trans[OF sym])
+         apply (assumption)
+        apply (erule arg_cong)
+(*repeat for each lin_pos *)
+       apply (rule conjI; (rule subprems)?)+
+        apply (rule subsetI)
+        apply (erule imageE)
+        apply (rule CollectI)
+        apply (rule case_prodI2)
         apply (drule trans[OF sym, THEN iffD1[OF prod.inject]])
          apply (assumption)
         apply (erule conjE)
@@ -1258,15 +936,8 @@ lemma F'_strong:
     and "rrel_F' Q x x'"
   shows "rrel_F' (inf R Q) x x'" 
   using assms apply -
-  apply (tactic \<open>mk_strong_tac @{thm rrel_F'_def} @{thm mr_rel_F_def} @{thm F_strong} @{thm F.map_id} @{context} 
-    THEN print_tac @{context} "done" THEN no_tac\<close>)
-  subgoal premises prems
-    apply (unfold rrel_F'_def)
-    apply (rule F_strong[unfolded mr_rel_F_def F.map_id, 
-          OF prems(1)[unfolded rrel_F'_def] prems(2)[unfolded rrel_F'_def], 
-          unfolded inf.idem])
-    done
-  done
+  by (tactic \<open>mk_strong_tac @{thm rrel_F'_def} @{thm mr_rel_F_def} @{thm F_strong} @{thm F.map_id} @{context} 
+    THEN print_tac @{context} "done"\<close>)
 
 ML \<open>
 open BNF_Util BNF_Tactics
@@ -1300,18 +971,12 @@ fun mk_is_mrbnf_tac F'_map_id F'_map_comp1 F'_map_cong F'_set1_map F'_set2_map F
     ) ctxt)
 \<close>
 
-mrbnf "('a::var, 'b::var, 'c::var, 'd) F'"
+mrbnf "('a::var, 'b::var, 'c::var, 'd, 'e::var) F'"
   map: map_F'
-  sets: free: set1_F' bound: set2_F' bound: set3_F' live: set4_F'
+  sets: free: set1_F' bound: set2_F' bound: set3_F' live: set4_F' bound: set5_F'
   bd: natLeq
   rel: rrel_F'
   var_class: var
-               apply (tactic \<open>mk_is_mrbnf_tac 
-  @{thm F'_map_id} @{thm F'_map_comp1_} @{thm F'_map_cong_}
-  @{thm F'_set1_map_} @{thm F'_set2_map_} @{thm F'_set3_map_} @{thm F'_set4_map_}
-  @{thm F'_set1_bd} @{thm F'_set2_bd} @{thm F'_set3_bd} @{thm F'_set4_bd}
-  @{thm F'_rel_comp_leq_} @{thm F'_in_rel} @{context}
-   THEN print_tac @{context} "done" THEN no_tac\<close>)
   subgoal by (rule F'_map_id)
   subgoal premises prems by (rule F'_map_comp1_; (rule prems))
   subgoal premises prems 
@@ -1333,11 +998,16 @@ mrbnf "('a::var, 'b::var, 'c::var, 'd) F'"
     apply (rule ext)
     apply (unfold o_apply F'_set4_map_[OF prems]) 
     by(rule refl)
+  subgoal premises prems 
+    apply (rule ext)
+    apply (unfold o_apply F'_set5_map_[OF prems]) 
+    by(rule refl)
   subgoal by (rule infinite_regular_card_order_natLeq)
   subgoal by (rule F'_set1_bd)
   subgoal by (rule F'_set2_bd)
   subgoal by (rule F'_set3_bd)
   subgoal by (rule F'_set4_bd)
+  subgoal by (rule F'_set5_bd)
   subgoal by (rule F'_rel_comp_leq_)
   subgoal premises prems by (rule F'_in_rel[OF prems])
   done        
